src/core/DY.Core.List.fst
@@ -1,0 +1,71 @@
+module DY.Core.List
+
+module List = FStar.List.Tot.Base
+
+let rec choose_equals (#a #b:eqtype) (f g: a -> option b) (xs: list a):
+  Lemma 
+  ( requires
+      forall x. x `List.mem` xs ==> f x = g x
+  )
+  (ensures
+    List.choose f xs = List.choose g xs
+  )
+  = normalize_term_spec (List.choose #a #b);
+    match xs with
+    | [] -> ()
+    | hd :: tl -> choose_equals f g tl
+
+
+
+let rec mem_choose (#a #b:eqtype) (f: a -> option b) (xs : list a) (x:a):
+  Lemma
+  (requires 
+     x `List.mem` xs /\ Some? (f x)
+  )
+  (ensures Some?.v (f x) `List.mem` (List.choose f xs)
+  )
+  = match xs with
+  | [] -> ()
+  | hd :: tl ->
+      if hd = x
+      then ()
+      else mem_choose f tl x 
+
+
+let rec mem_choose_elim (#a #b:eqtype) (f: a -> option b) (xs : list a) (y : b)
+  : Lemma
+  (ensures (
+    y `List.mem` (List.choose f xs) ==> 
+    (exists x. x `List.mem` xs /\ Some? (f x) /\ Some?.v (f x) = y)
+    )
+  )
+  =match xs with
+  | [] -> ()
+  | hd :: tl -> mem_choose_elim f tl y
+
+
+let rec mem_index (#a:eqtype) (xs: list a) (x:a):
+  Lemma
+  (requires
+    x `List.mem` xs
+  )
+  (ensures (exists i. x = List.index xs i)
+  )
+  = match xs with
+  | [] -> ()
+  | hd :: tl -> 
+    if hd = x 
+    then (
+      introduce exists i. x = List.index xs i
+      with 0
+      and ()
+    )
+    else ( 
+      mem_index tl x;
+      eliminate exists i. x = List.index tl i
+      returns (exists i. x = List.index xs i)
+      with _ .
+      ( introduce exists i. x = List.index xs i
+        with (i+1) and ()
+      )
+    )
