src/core/DY.Core.Trace.PrefixSuffix.fst
@@ -1,0 +1,256 @@
+module DY.Core.Trace.PrefixSuffix
+
+open  DY.Core.Trace.Type
+module Trace = DY.Core.Trace.Type
+open DY.Core.Bytes.Type
+open DY.Core.Label.Type
+
+
+let rec prefix_including_event (tr:trace) (the_ev:trace_event{event_exists tr the_ev}) =
+  match tr with
+  | Snoc init ev ->
+      if ev = the_ev 
+        then tr
+        else init `prefix_including_event` the_ev
+
+let rec prefix_including_event_is_prefix (tr:trace) (the_ev:trace_event{event_exists tr the_ev}) :
+  Lemma (tr `prefix_including_event` the_ev <$ tr)
+  [SMTPat (tr `prefix_including_event` the_ev)] =
+  reveal_opaque (`%grows) grows; 
+  norm_spec [zeta; delta_only [`%prefix]] (prefix);
+  match tr with
+  | Nil -> ()
+  | Snoc init ev ->
+         if ev = the_ev
+           then ()
+           else
+             prefix_including_event_is_prefix init the_ev
+
+
+/// definition of "trace substraction"
+/// (it holds: tr2 = tr1 ++ tr2 `suffix_after` tr1)
+
+val suffix_after: tr2:trace -> tr1:trace{tr1 <$ tr2} -> trace
+let rec suffix_after tr2 tr1 = 
+  match tr2 with
+  | Nil -> Nil
+  | Snoc init ev -> 
+      if length tr2 = length tr1
+        then Nil
+        else begin 
+             reveal_opaque (`%grows) grows; 
+             norm_spec [zeta; delta_only [`%prefix]] (prefix);
+             Snoc (suffix_after init tr1) ev
+         end
+
+val suffix_after_splits_trace:
+  tr2:trace -> tr1:trace{tr1 <$ tr2} ->
+  Lemma (tr2 = tr1 `trace_concat` (tr2 `suffix_after` tr1))
+let rec suffix_after_splits_trace tr2 tr1 =
+  reveal_opaque (`%grows) grows; 
+  norm_spec [zeta; delta_only [`%prefix]] (prefix);
+  match tr2 with
+  | Nil -> ()
+  | Snoc init ev -> 
+         if length tr1 = length tr2 
+           then ()
+           else suffix_after_splits_trace init tr1
+
+
+
+/// for traces with tr1 <$ tr2 <$ tr3,
+/// the suffix after tr1 on tr2
+/// is a prefix of
+/// the suffix after tr1 on tr3
+
+val suffix_after_for_prefix: 
+  tr3:trace -> tr2:trace {tr2 <$ tr3} -> tr1:trace {tr1 <$ tr2} ->
+  Lemma 
+    (tr2 `suffix_after` tr1 <$ tr3 `suffix_after` tr1)
+let rec suffix_after_for_prefix tr3 tr2 tr1 = 
+  reveal_opaque (`%grows) grows; 
+  norm_spec [zeta; delta_only [`%prefix]] (prefix);
+  if length tr3 = length tr2 || length tr2 = length tr1
+    then ()
+    else begin
+      match tr3 with
+      | Nil -> ()
+      | Snoc init ev -> suffix_after_for_prefix init tr2 tr1
+    end
+
+
+  
+/// for traces with tr1 <$ tr2 <$ tr3,
+/// the suffix after tr1 on tr3
+/// is the concat of the two pairwise suffixes
+#push-options "--fuel 2"
+val suffix_after_concat:
+  tr1:trace -> tr2:trace {tr1 <$ tr2} -> tr3:trace{tr2 <$ tr3} ->
+  Lemma
+  ( tr3 `suffix_after` tr1 == (tr2 `suffix_after` tr1) `trace_concat` (tr3 `suffix_after` tr2)
+  )
+let rec suffix_after_concat tr1 tr2 tr3 =     
+  reveal_opaque (`%grows) (grows);
+  norm_spec [zeta; delta_only [`%prefix]] (prefix);
+  match tr3 with
+  | Nil -> ()
+  | Snoc init ev -> 
+      if length tr2 = length tr3
+        then ()
+        else suffix_after_concat tr1 tr2 init
+#pop-options
+
+let suffix_after_event (tr:trace) (ev:trace_event{event_exists tr ev}) =
+  let tr_before = tr `prefix_including_event` ev in
+  tr `suffix_after` tr_before
+
+
+let rec suffix_after_event_init
+  (tr:trace{Snoc? tr}) (the_ev:trace_event{event_exists tr the_ev})
+  :Lemma 
+    ( let Snoc init ev = tr in
+      if the_ev <> ev
+        then tr `suffix_after_event` the_ev = Snoc (init `suffix_after_event` the_ev) ev
+        else True
+    )
+= let Snoc init ev = tr in
+  if the_ev <> ev
+    then
+      suffix_after_event_init init the_ev
+    else ()
+
+
+let rec has_suffix (tr:trace) (suff:trace) =
+  match suff with
+  | Nil -> true
+  | Snoc suff_init suff_ev ->
+      match tr with
+      | Nil -> false
+      | Snoc tr_init tr_ev ->
+          suff_ev = tr_ev && (has_suffix tr_init suff_init)
+
+let _ = 
+  let ev1 = Corrupt "p" {the_id = 1} in 
+  let ev2 = Corrupt "p" {the_id = 2} in 
+  let ev3 = Corrupt "p" {the_id = 3} in 
+  let tr = Snoc (Snoc (Snoc Nil ev1) ev2) ev3 in
+  let tr' = Snoc (Snoc Nil ev2) ev3 in
+  assert(tr `has_suffix` tr')
+
+
+let rec suffix_after_is_suffix (tr:trace) (pref:trace{pref <$ tr}):
+  Lemma
+  (tr `has_suffix` (tr `suffix_after` pref)
+  )
+  [SMTPat (tr `has_suffix` (tr `suffix_after` pref))]
+  =
+  let suff = tr `suffix_after` pref in
+  match suff with
+  | Nil -> ()
+  | Snoc suff_init suff_ev ->
+         match tr with
+         | Nil -> ()
+         | Snoc tr_init tr_ev -> 
+                assert(suff_ev = tr_ev);
+                init_is_prefix tr;
+                reveal_opaque (`%grows) grows; 
+                suffix_after_is_suffix (tr_init) pref
+
+
+
+let rec suffixes_ (tr:trace) (suff1:trace) (suff2:trace):
+  Lemma
+  (requires
+      tr `has_suffix` suff1
+    /\ tr `has_suffix` suff2
+    /\ Trace.length suff1 >= Trace.length suff2
+  )
+  (ensures
+        suff1 `has_suffix` suff2 
+  )
+  = match suff2 with
+  | Nil -> ()
+  | Snoc init2 last2 -> 
+      let Snoc init1 last1 = suff1 in
+      let Snoc init last = tr in 
+      suffixes_ init init1 init2
+
+let suffixes (tr:trace) (suff1:trace) (suff2:trace):
+  Lemma
+  (requires
+      tr `has_suffix` suff1
+    /\ tr `has_suffix` suff2
+  )
+  (ensures
+        suff1 `has_suffix` suff2 
+      \/ suff2 `has_suffix` suff1
+  )
+  = if Trace.length suff1 >= Trace.length suff2
+       then suffixes_ tr suff1 suff2
+       else suffixes_ tr suff2 suff1
+
+
+let rec suffix_after_nil (tr:trace):
+  Lemma (tr `suffix_after` Nil = tr)
+  [SMTPat (tr `suffix_after` Nil)]
+  = match tr with
+    | Nil -> ()
+    | Snoc init ev -> suffix_after_nil init
+
+
+let prepend  (ev:trace_event) (tr:trace) =
+  (Snoc Nil ev) `trace_concat` tr
+
+
+
+let rec event_splits_trace (tr:trace) (ev:trace_event{event_exists tr ev}):
+  Lemma
+  ( let tr_before = tr `prefix_before_event` ev in
+    let tr_after = tr `suffix_after_event` ev in
+    tr = tr_before `trace_concat` (prepend ev tr_after)
+  )
+  = let tr_before = tr `prefix_before_event` ev in
+    let tr_after = tr `suffix_after_event` ev in
+    match tr with
+    | Nil -> ()
+    | Snoc tr_init tr_last ->
+        if tr_last = ev
+          then ()
+          else event_splits_trace tr_init ev
+        
+
+let suffix_after_snoc (init:trace) (ev:trace_event) (pref:trace{pref <$ init}):
+  Lemma
+  ( reveal_opaque (`%grows) grows; 
+    norm_spec [zeta; delta_only [`%prefix]] (prefix);
+
+    (Snoc init ev) `suffix_after` pref = Snoc ( init `suffix_after` pref ) ev
+  )
+= normalize_term_spec suffix_after
+
+let rec suffix_after_concat_ (pref:trace) (suff:trace):
+  Lemma 
+  ( let tr = pref `trace_concat` suff in
+    trace_concat_grows pref suff;
+    tr `suffix_after` pref = suff
+  )
+  = 
+  let tr = pref `trace_concat` suff in
+  match suff with
+  | Nil -> ()
+  | Snoc suff_init suff_ev ->
+         suffix_after_concat_ pref suff_init;
+         trace_concat_grows pref suff_init;
+         suffix_after_snoc ( pref `trace_concat` suff_init  ) suff_ev pref
+
+let suff_after_before_event_is_suff_at_event (tr:trace) (ev:trace_event{event_exists tr ev}):
+  Lemma
+  ( let tr_before = tr `prefix_before_event` ev in
+    let tr_after = tr `suffix_after_event` ev in
+    tr `suffix_after` tr_before = (Snoc Nil ev) `trace_concat` tr_after
+  )
+  = let tr_before = tr `prefix_before_event` ev in
+    let tr_after = tr `suffix_after_event` ev in
+    event_splits_trace tr ev;
+    suffix_after_concat_ tr_before (prepend ev tr_after)
+    
