src/core/DY.Core.Trace.State.Properties.fst
@@ -1,0 +1,494 @@
+module DY.Core.Trace.State.Properties
+
+open FStar.List.Tot
+
+open DY.Core.Bytes.Type
+open DY.Core.Bytes
+open DY.Core.Label.Type
+open DY.Core.Trace.Type
+open DY.Core.Trace.PrefixSuffix
+open DY.Core.Trace.State.Aux
+open DY.Core.Trace.Manipulation
+open DY.Core.List
+
+module List = FStar.List.Tot.Base
+
+
+
+let no_set_state_entry_for_p (p:principal) (tr:trace) =
+  forall sid. no_set_state_entry_for p sid tr
+
+let rec compute_new_session_id_same (p:principal) (tr1 tr2:trace) :
+  Lemma (
+    requires
+      tr1 <$ tr2 /\ 
+      no_set_state_entry_for_p p (tr2 `suffix_after` tr1)
+  )
+  (ensures
+    compute_new_session_id p tr1 = compute_new_session_id p tr2
+  )
+  = reveal_opaque (`%grows) grows; 
+    norm_spec [zeta; delta_only [`%prefix]] (prefix);
+    if tr1 = tr2 
+    then ()
+    else (
+      match tr2 with
+       | Nil -> ()
+       | Snoc init (SetState p' sid' cont') -> (
+           let ev = (SetState p' sid' cont') in
+           assert(event_exists (tr2 `suffix_after` tr1) ev);
+           suffix_after_for_prefix tr2 init tr1;
+           compute_new_session_id_same p tr1 init
+         )
+       | Snoc init ev -> 
+           suffix_after_for_prefix tr2 init tr1;
+           compute_new_session_id_same p tr1 init
+    )
+
+
+let rec zero_to_sid_mem (bound:state_id) (x :state_id{x.the_id <= bound.the_id}):
+  Lemma ( ensures
+    x `List.mem` (zero_to_sid bound)
+  )
+  (decreases bound.the_id)  
+  = if bound.the_id = 0
+    then ()
+    else begin
+      FStar.List.Tot.Properties.append_mem_forall (zero_to_sid {the_id = bound.the_id - 1}) [bound];
+      if x = bound
+      then ()
+      else 
+        zero_to_sid_mem ({the_id = bound.the_id -1}) x
+    end
+
+
+let rec zero_to_sid_mems (bound:state_id) (sid:state_id) :
+  Lemma 
+  (requires
+    sid `List.mem` (zero_to_sid bound)
+  )
+  ( ensures
+  sid.the_id <= bound.the_id
+  )
+  (decreases bound.the_id)
+  = if bound.the_id = 0
+    then ()
+    else (
+      if sid = bound
+      then ()
+      else (
+     FStar.List.Tot.Properties.append_mem_forall (zero_to_sid {the_id = bound.the_id - 1}) [bound];
+     zero_to_sid_mems ({the_id =bound.the_id - 1}) sid
+     )
+  )
+
+
+let get_full_state_same (p:principal) (tr1:trace) (tr2:trace):
+  Lemma
+  (requires
+      tr1 <$ tr2 /\ 
+      no_set_state_entry_for_p p (tr2 `suffix_after` tr1)
+    )
+  (ensures get_full_state p tr1 = get_full_state p tr2)
+= introduce forall sid. get_session_indexed tr1 p sid = get_session_indexed tr2 p sid
+  with (
+    reveal_opaque (`%get_session) get_session; 
+    get_session_aux_same p sid tr1 tr2
+  ); 
+  compute_new_session_id_same p tr1 tr2;
+  choose_equals
+    (get_session_indexed tr1 p) 
+    (get_session_indexed tr2 p) 
+    (zero_to_sid (compute_new_session_id p tr1))
+  
+
+
+let rec compute_new_session_id_grows (p:principal) (tr1 tr2:trace):
+  Lemma 
+  (requires tr1 <$ tr2
+  )
+  (ensures
+    (compute_new_session_id p tr1).the_id <= (compute_new_session_id p tr2).the_id
+  )
+  = reveal_opaque (`%grows) grows; 
+    norm_spec [zeta; delta_only [`%prefix]] (prefix);
+    if tr1 = tr2
+    then ()
+    else (
+      match tr2 with
+      | Nil -> ()
+      | Snoc tr2_init tr2_ev -> compute_new_session_id_grows p tr1 tr2_init
+    )
+
+
+
+val full_state_session_lemma:
+  (tr:trace) -> (p:principal) -> (i:nat) ->
+  Lemma(
+    match get_full_state p tr with 
+      | None -> True
+      | Some full_st -> begin
+          if i >= List.length full_st
+            then True
+            else begin
+              let (sid_i, sess_i) = List.index full_st i in
+              get_session p sid_i tr = Some sess_i
+            end
+      end
+  )
+let full_state_session_lemma tr p i =
+    match get_full_state p tr with 
+      | None -> ()
+      | Some full_st -> begin
+          if i >= List.length full_st
+            then ()
+            else (
+              let (sid_i, sess_i) = List.index full_st i in
+              let next_sid = compute_new_session_id p tr in
+              let sids = zero_to_sid next_sid in
+              let f = get_session_indexed tr p in
+              FStar.List.Tot.Properties.lemma_index_memP full_st i;
+              mem_choose_elim f sids (sid_i, sess_i)
+              )
+      end
+
+
+let full_state_some_get_session_some (p:principal) (sid:state_id) (tr:trace):
+  Lemma 
+  (requires
+     Some? (get_full_state p tr)
+     /\ sid `List.mem` (List.map fst (Some?.v (get_full_state p tr)))
+  )
+  (ensures
+     Some? (get_session p sid tr)
+  )
+  = let Some full_st = get_full_state p tr in
+    let next_sid = compute_new_session_id p tr in
+    let sids = zero_to_sid next_sid in
+    FStar.List.Tot.Properties.memP_map_elim fst sid full_st;
+    eliminate exists sess. (sid, sess) `List.mem` full_st 
+    returns Some? (get_session p sid tr)
+    with _ .
+      mem_choose_elim (get_session_indexed tr p) sids (sid, sess)
+    
+
+
+let rec get_session_grows (p:principal) (sid:state_id) (tr1 tr2:trace):
+  Lemma
+  ( requires tr1 <$ tr2 /\ Some? (get_session p sid tr1)
+  )
+  (ensures
+    Some? (get_session p sid tr2)
+  )
+ = reveal_opaque (`%grows) grows; 
+   norm_spec [zeta; delta_only [`%prefix]] (prefix);
+   if tr1 = tr2 
+   then ()
+   else (
+     match tr2 with
+     | Nil -> ()
+     | Snoc init _ -> get_session_grows p sid tr1 init
+   )
+
+
+
+let rec get_session_state_was_set (p:principal) (sid:state_id) (tr:trace):
+  Lemma
+  (requires Some? (get_session p sid tr))
+  (ensures exists cont. state_was_set tr p sid cont )
+  = match tr with
+  | Nil -> ()
+  | Snoc init (SetState p' sid' cont') -> (
+         if p' = p && sid' = sid
+         then ()
+         else get_session_state_was_set p sid init
+   )      
+  | Snoc init _ -> 
+        get_session_state_was_set p sid init
+
+
+
+let get_session_some_full_state_some (p:principal) (sid:state_id) (tr:trace):
+  Lemma 
+  ( requires Some? (get_session p sid tr)
+  )
+  (ensures Some? (get_full_state p tr)
+  )
+  =
+    get_session_state_was_set p sid tr;
+    eliminate exists cont . state_was_set tr p sid cont
+    returns Some? (get_full_state p tr)
+    with _ .
+        compute_new_session_id_larger_than_id_on_trace p tr sid cont
+
+
+let full_state_fst_zero_to_sid (tr:trace) (p:principal):
+  Lemma
+  ( requires Some? (get_full_state p tr)
+  )
+  (ensures (
+    let Some full_st = get_full_state p tr in
+    let next_sid = compute_new_session_id p tr in
+    (List.map fst (full_st)) `List.subset` (zero_to_sid next_sid)
+    )
+  )
+  =
+    let Some full_st = get_full_state p tr in
+    let next_sid = compute_new_session_id p tr in
+  introduce forall sid. sid `List.mem` (List.map fst full_st) ==> sid `List.mem` (zero_to_sid next_sid)
+  with (
+    introduce _ ==> _
+    with _ . (
+      FStar.List.Tot.Properties.memP_map_elim fst sid full_st;
+      eliminate exists sess. (sid, sess) `List.mem` full_st
+      returns _
+      with _ . (
+      mem_choose_elim (get_session_indexed tr p) (zero_to_sid next_sid) (sid,sess)      
+      )
+    )
+  )
+
+
+
+let get_full_state_on_growing_traces (p:principal) (tr1 tr2:trace) (sid:state_id):
+  Lemma 
+  (requires
+      tr1 <$ tr2
+    /\ Some? (get_full_state p tr1)
+    /\ sid `List.mem` (List.map fst (Some?.v (get_full_state p tr1)))
+  )
+  (ensures
+    Some? (get_full_state p tr2) /\    
+    sid `List.mem` (List.map fst (Some?.v (get_full_state p tr2)))
+  )
+  = 
+  let Some full_st1 = get_full_state p tr1 in
+ 
+         let new_sid1 = compute_new_session_id p tr1 in
+         let new_sid2 = compute_new_session_id p tr2 in
+         compute_new_session_id_grows p tr1 tr2;
+         let sids1 = zero_to_sid new_sid1 in
+         let sids2 = zero_to_sid new_sid2 in
+         full_state_fst_zero_to_sid tr1 p;
+           zero_to_sid_mems new_sid1 sid;
+           zero_to_sid_mem new_sid2 sid;
+         
+         full_state_some_get_session_some p sid tr1;
+         get_session_grows p sid tr1 tr2;
+         let Some sess2 = get_session p sid tr2 in
+         get_session_some_full_state_some p sid tr2;
+         let Some full_st2 = get_full_state p tr2 in
+         mem_choose (get_session_indexed tr2 p) sids2 sid;
+         FStar.List.Tot.Properties.memP_map_intro fst (sid, sess2) full_st2
+   
+
+let rec state_was_set_full_state (tr:trace) (p:principal) (sid:state_id) (cont:bytes):
+  Lemma
+  (requires
+    state_was_set tr p sid cont
+  )
+  (ensures
+    Some? (get_full_state p tr) 
+    /\ sid `List.mem` (List.map fst (Some?.v (get_full_state p tr)))
+  )
+= match tr with
+  | Nil -> ()
+  | Snoc init (SetState p' sid' cont') ->
+      if p' = p 
+        then ( 
+        if sid' = sid
+        then (
+          compute_new_session_id_larger_than_id_on_trace p tr sid cont';
+          zero_to_sid_mem (compute_new_session_id p tr) sid;
+          assert(Some? (get_session p sid tr));
+          let f = get_session_indexed tr p in
+          let sids = (zero_to_sid (compute_new_session_id p tr)) in
+          let Some full_st = get_full_state p tr in
+          mem_choose f sids sid;
+          FStar.List.Tot.Properties.memP_map_intro fst (sid, Some?.v (get_session p sid tr)) full_st
+          )
+          else (
+          init_is_prefix tr;
+          state_was_set_full_state init p sid cont;
+          get_full_state_on_growing_traces p init tr sid
+          )
+        )
+        else (
+          init_is_prefix tr;
+          get_full_state_same p init tr;
+          state_was_set_full_state init p sid cont
+        ) 
+ | Snoc init _ -> 
+     init_is_prefix tr;
+     get_full_state_same p init tr;
+     state_was_set_full_state init p sid cont
+
+
+val parse_full_state_lemma :
+  (tr: trace) -> p:principal -> (i:nat) ->
+  Lemma 
+    (
+      match get_full_state p tr with 
+      | None -> True
+      | Some full_st -> begin
+          if i >= List.length full_st
+            then True
+            else begin
+                   match List.index full_st i with
+                   | (_, Nil) -> True
+                   | (sid_i, (Snoc init_i last_i)) -> begin
+                         Some?   (fst (get_state p sid_i tr))
+                       /\ Some?.v (fst (get_state p sid_i tr)) = last_i
+                   end
+            end
+      end
+      
+    )
+let parse_full_state_lemma tr p i =
+  reveal_opaque (`%get_state) get_state;
+      match get_full_state p tr with 
+      | None -> ()
+      | Some full_st -> begin
+          if i >= List.length full_st
+            then ()
+            else begin
+                   match List.index full_st i with
+                   | (_, Nil) -> ()
+                   | (sid_i, (Snoc init_i last_i)) -> begin
+                       full_state_session_lemma tr p i
+                   end
+            end
+      end 
+
+
+val get_state_appears_in_full_state_ :
+  tr:trace -> p:principal -> sid:state_id ->
+  Lemma
+  (requires
+     Some? (fst (get_state p sid tr))
+     /\ Some? (get_full_state p tr)
+  )
+  (ensures (
+    let (Some state, _) = get_state p sid tr in
+    let Some full_state = get_full_state p tr in
+    
+    exists init. (sid, Snoc init state) `List.mem` full_state 
+  )
+  )
+let get_state_appears_in_full_state_  tr p sid =
+  let (Some state, _) = get_state p sid tr in
+  let Some full_state = get_full_state p tr in
+  state_was_set_full_state tr p sid state;
+  FStar.List.Tot.Properties.memP_map_elim fst sid full_state;
+  
+  let Some session = get_session p sid tr in
+  eliminate exists sess. (sid, sess) `List.mem` full_state
+  returns (sid, session) `List.mem` full_state
+  with _ . (
+    mem_index full_state (sid, sess);
+    eliminate exists i . (sid, sess) = List.index full_state i
+    returns _
+    with _ . (
+      full_state_session_lemma tr p i;
+    ()
+    )
+  );  
+  ()
+
+
+val get_state_appears_in_full_state :
+  tr:trace -> p:principal -> sid:state_id ->
+  Lemma
+  ( 
+    match get_state p sid tr with
+    | (None, _) -> True
+    | (Some state, _) -> (
+        match get_full_state p tr with
+        | None -> True
+        | Some full_state ->
+            exists i init . List.index full_state i = (sid, Snoc init state)
+            )
+  )
+let get_state_appears_in_full_state  tr p sid =
+    match get_state p sid tr with
+    | (None, _) -> ()
+    | (Some state, _) -> (
+        match get_full_state p tr with
+        | None -> ()
+        | Some full_state -> (
+          get_state_appears_in_full_state_ tr p sid;
+          eliminate exists init . (sid, Snoc init state) `List.mem` full_state
+          returns exists i init . List.index full_state i = (sid, Snoc init state)
+          with _ . (
+            mem_index full_state (sid, Snoc init state)
+          );
+          // assert(exists i init . List.index full_state i = (sid, Snoc init state))
+          admit() /// ??? WHY ??? the above assert works fine...
+          )
+          )
+
+
+val get_state_get_full_state:
+  p:principal -> sid:state_id -> tr:trace ->
+  Lemma 
+    (requires True
+    )
+    (ensures (
+      let (opt_state, _) = get_state p sid tr in
+      let opt_full_state = get_full_state p tr in
+      match opt_state with
+      | None -> True
+      | Some st -> 
+          Some? opt_full_state
+    )
+    )
+let get_state_get_full_state p sid tr =
+    let (opt_state, _) = get_state p sid tr in
+      match opt_state with
+      | None -> ()
+      | Some st -> state_was_set_full_state tr p sid st
+
+
+let rec get_state_no_set_state_for_on_suffix_after_event
+  (tr:trace) (p:principal) (sid:state_id) :
+  Lemma 
+  ( let (opt_cont, tr_out) = get_state p sid tr in
+  match opt_cont with
+    | None -> True
+    | Some st -> no_set_state_entry_for p sid (tr `suffix_after_event` (SetState p sid st)) 
+  )
+  = reveal_opaque (`%get_state) get_state; 
+  match get_state p sid tr with
+  | (None, _) -> ()
+  | (Some st, _) ->
+  match tr with
+  | Nil -> ()
+  | Snoc init (SetState p' sid' cont') -> 
+         if p' = p && sid' = sid
+           then ()
+           else ( 
+             get_state_no_set_state_for_on_suffix_after_event init p sid;
+             suffix_after_event_init tr (SetState p' sid' cont')
+           )
+  | Snoc init ev -> 
+    get_state_no_set_state_for_on_suffix_after_event init p sid;
+    suffix_after_event_init tr (SetState p sid st)
+
+
+let rec no_set_state_entry_for_on_suffix (tr:trace) (suff:trace) (p:principal) (sid:state_id):
+  Lemma
+  (requires tr `has_suffix` suff /\ no_set_state_entry_for p sid tr
+  )
+  (ensures
+    no_set_state_entry_for p sid suff
+  )
+  = match suff with
+  | Nil -> ()
+  | Snoc suff_init suff_ev ->
+         match tr with
+         | Nil -> ()
+         | Snoc tr_init tr_ev -> 
+                init_is_prefix tr;
+                no_set_state_entry_for_on_suffix tr_init suff_init p sid;
+                assert(event_exists tr tr_ev)
+
